Corrected interface

mrdts-new/Enable_wins_flag/App.fst
@@ -1,183 +1,208 @@
 module App
 
-open FStar.Seq
+module M = Map_extended
+module S = Set_extended
+
+#set-options "--query_stats"
+
+let cf = (int * bool)
 
 // the concrete state type
-val concrete_st : Type0
+type concrete_st = M.t nat cf // (replica_id, ctr, flag) //replica ids are unique
+
+let sel (s:concrete_st) k = if M.contains s k then M.sel s k else (0, false)
 
 // init state
-val init_st : concrete_st
+let init_st : concrete_st = M.const (0, false)
 
 // equivalence between 2 concrete states
-val eq (a b:concrete_st) : Type0
+let eq (a b:concrete_st) =
+  (forall id. (M.contains a id = M.contains b id) /\ (sel a id == sel b id))
 
-val symmetric (a b:concrete_st) 
+let symmetric (a b:concrete_st) 
   : Lemma (requires eq a b)
-          (ensures eq b a)
+          (ensures eq b a) = ()
 
-val transitive (a b c:concrete_st)
+let transitive (a b c:concrete_st)
   : Lemma (requires eq a b /\ eq b c)
-          (ensures eq a c)
+          (ensures eq a c) = ()
 
-val eq_is_equiv (a b:concrete_st)
+let eq_is_equiv (a b:concrete_st)
   : Lemma (requires a == b)
-          (ensures eq a b)
+          (ensures eq a b) = ()
 
 // operation type
-val app_op_t : eqtype 
-
-type op_t = pos (*timestamp*) & (nat (*replica ID*) & app_op_t)
-
-let get_rid (_,(rid,_)) = rid
-
-let distinct_ops (op1 op2:op_t) = fst op1 =!= fst op2
-
-type log = seq op_t
+type app_op_t:eqtype =
+  |Enable 
+  |Disable
 
 // apply an operation to a state
-val do (s:concrete_st) (o:op_t) : concrete_st
-
-let commutes_with (o1 o2:op_t) =
-  forall s. eq (do (do s o1) o2) (do (do s o2) o1)
-
-// applying a log of operations to a concrete state
-let rec apply_log (x:concrete_st) (l:log) : Tot concrete_st (decreases length l) =
-  match length l with
-  |0 -> x
-  |_ -> apply_log (do x (head l)) (tail l)  
-  
-//conflict resolution type
-type rc_res =
-  |Fst_then_snd //o1 -> o2
-  |Snd_then_fst //o2 -> o1
-  |Either
+let do (s:concrete_st) (o:op_t) : concrete_st =
+  match o with
+  |(_, (rid, Enable)) -> M.upd s rid (fst (sel s rid) + 1, true)
+  |(_, (rid, Disable)) -> M.map_val (fun (c,f) -> (c, false)) s
 
 //conflict resolution
-val rc (o1 o2:op_t) : rc_res
+let rc (o1 o2:op_t) =
+  match snd (snd o1), snd (snd o2) with
+  |Enable, Disable -> Snd_then_fst
+  |Disable, Enable -> Fst_then_snd 
+  |_ -> Either
+
+let merge_flag (l a b:cf) : bool =
+  let lc = fst l in
+  let ac = fst a in
+  let bc = fst b in
+  let af = snd a in
+  let bf = snd b in
+    if af && bf then true
+      else if not af && not bf then false
+        else if af then ac > lc
+          else bc > lc
 
 // concrete merge operation
-val merge (l a b:concrete_st) : concrete_st
+let merge_cf (l a b:cf) : cf =
+  (fst a + fst b - fst l, merge_flag l a b)
+  
+// concrete merge operation
+let merge (l a b:concrete_st) : concrete_st =
+  let keys = S.union (M.domain l) (S.union (M.domain a) (M.domain b)) in
+  let u = M.const_on keys (0, false) in
+  M.iter_upd (fun k v -> merge_cf (sel l k) (sel a k) (sel b k)) u
 
 /////////////////////////////////////////////////////////////////////////////
 
-val rc_non_comm (o1 o2:op_t)
+let rc_non_comm_help1 (o1 o2:op_t)
   : Lemma (requires distinct_ops o1 o2)
-          (ensures Either? (rc o1 o2) <==> commutes_with o1 o2)
-
-val no_rc_chain (o1 o2 o3:op_t)
+          (ensures ((Enable? (snd (snd o1)) /\ Disable? (snd (snd o2))) ==> ~ (eq (do (do init_st o1) o2) (do (do init_st o2) o1)))) = ()
+         
+let rc_non_comm_help2 (o1 o2:op_t)
+  : Lemma (requires distinct_ops o1 o2)
+          (ensures ((Disable? (snd (snd o1)) /\ Enable? (snd (snd o2))) ==> ~ (eq (do (do init_st o1) o2) (do (do init_st o2) o1)))) = ()
+          
+let rc_non_comm (o1 o2:op_t)
+  : Lemma (requires distinct_ops o1 o2)
+          (ensures Either? (rc o1 o2) <==> commutes_with o1 o2) = 
+  rc_non_comm_help1 o1 o2;
+  rc_non_comm_help2 o1 o2
+          
+let no_rc_chain (o1 o2 o3:op_t)
   : Lemma (requires distinct_ops o1 o2 /\ distinct_ops o2 o3)
-          (ensures ~ (Fst_then_snd? (rc o1 o2) /\ Fst_then_snd? (rc o2 o3)))
+          (ensures ~ (Fst_then_snd? (rc o1 o2) /\ Fst_then_snd? (rc o2 o3))) = ()
 
-val cond_comm_base (s:concrete_st) (o1 o2:op_t) (o3:op_t{distinct_ops o1 o2 /\ distinct_ops o1 o3 /\ distinct_ops o2 o3})
-    : (b:bool{(Fst_then_snd? (rc o1 o2) /\ ~ (Either? (rc o2 o3))) ==> eq (do (do (do s o1) o2) o3) (do (do (do s o2) o1) o3)})
+let cond_comm_base (s:concrete_st) (o1 o2:op_t) (o3:op_t{distinct_ops o1 o2 /\ distinct_ops o1 o3 /\ distinct_ops o2 o3})
+    : (b:bool{(Fst_then_snd? (rc o1 o2) /\ ~ (Either? (rc o2 o3))) ==> eq (do (do (do s o1) o2) o3) (do (do (do s o2) o1) o3)}) = 
+    if Disable? (snd (snd o3)) then true else false
 
-val cond_comm_ind (s:concrete_st) (o1 o2 o3 o:op_t) (l:seq op_t)
+let cond_comm_ind (s:concrete_st) (o1 o2 o3 o:op_t) (l:seq op_t)
   : Lemma (requires distinct_ops o1 o2 /\ distinct_ops o1 o3 /\ distinct_ops o2 o3 /\ cond_comm_base s o1 o2 o3 /\
                     eq (do (apply_log (do (do s o1) o2) l) o3) (do (apply_log (do (do s o2) o1) l) o3))
-          (ensures eq (do (do (apply_log (do (do s o1) o2) l) o) o3) (do (do (apply_log (do (do s o2) o1) l) o) o3))
-                  
-////////////////////////////////////////////////////////////////////////////
+          (ensures eq (do (do (apply_log (do (do s o1) o2) l) o) o3) (do (do (apply_log (do (do s o2) o1) l) o) o3)) = ()
+ 
+/////////////////////////////////////////////////////////////////////////////
+// Merge commutativity
+let merge_comm (l a b:concrete_st)
+   : Lemma (ensures (eq (merge l a b) (merge l b a))) = ()
 
-val merge_comm (l a b:concrete_st)
-  : Lemma (ensures (eq (merge l a b) (merge l b a)))
-                       
-val merge_idem (s:concrete_st)
-  : Lemma (ensures eq (merge s s s) s)
+// Merge idempotence
+let merge_idem (s:concrete_st)
+   : Lemma (ensures eq (merge s s s) s) = ()
 
+#push-options "--z3rlimit 100 --max_ifuel 3"
 (*Two OP RC*)
 //////////////// 
-val rc_ind_right (l a b:concrete_st) (o1 o2 o2':op_t)
+let rc_ind_right (l a b:concrete_st) (o1 o2 o2':op_t)
   : Lemma (requires Fst_then_snd? (rc o1 o2) /\
                     distinct_ops o1 o2 /\ distinct_ops o1 o2' /\ distinct_ops o2 o2' /\  
                     eq (merge l (do a o1) (do b o2)) (do (merge l (do a o1) b) o2))
-          (ensures eq (merge l (do a o1) (do (do b o2') o2)) (do (merge l (do a o1) (do b o2')) o2))
+          (ensures eq (merge l (do a o1) (do (do b o2') o2)) (do (merge l (do a o1) (do b o2')) o2)) = ()
 
-val rc_ind_left (l a b:concrete_st) (o1 o2 o1':op_t)
+let rc_ind_left (l a b:concrete_st) (o1 o2 o1':op_t)
   : Lemma (requires Fst_then_snd? (rc o1 o2) /\
                     distinct_ops o1 o2 /\ distinct_ops o1 o1' /\ distinct_ops o2 o1' /\
                     eq (merge l (do a o1) (do b o2)) (do (merge l (do a o1) b) o2))
-          (ensures eq (merge l (do (do a o1') o1) (do b o2)) (do (merge l (do (do a o1') o1) b) o2))
+          (ensures eq (merge l (do (do a o1') o1) (do b o2)) (do (merge l (do (do a o1') o1) b) o2)) = ()
 
 //Special case of rc_intermediate_v1
-val rc_ind_lca (l:concrete_st) (o1 o2 o:op_t)
+let rc_ind_lca (l:concrete_st) (o1 o2 o:op_t)
   : Lemma (requires Fst_then_snd? (rc o1 o2) /\ 
                     distinct_ops o1 o2 /\ distinct_ops o o1 /\ distinct_ops o o2 /\
                     eq (merge l (do l o1) (do l o2)) (do (do l o1) o2))
-          (ensures eq (merge (do l o) (do (do l o) o1) (do (do l o) o2)) (do (do (do l o) o1) o2))
+          (ensures eq (merge (do l o) (do (do l o) o1) (do (do l o) o2)) (do (do (do l o) o1) o2)) = ()
 
-val rc_base (o1 o2:op_t)
+let rc_base (o1 o2:op_t)
   : Lemma (requires Fst_then_snd? (rc o1 o2) /\ distinct_ops o1 o2)
-          (ensures eq (merge init_st (do init_st o1) (do init_st o2)) (do (do init_st o1) o2))
+          (ensures eq (merge init_st (do init_st o1) (do init_st o2)) (do (do init_st o1) o2)) = ()
 
-val rc_inter_base_right (l a b c:concrete_st) (o1 o2 ob ol:op_t) 
+let rc_inter_base_right (l a b c:concrete_st) (o1 o2 ob ol:op_t) 
   : Lemma (requires Fst_then_snd? (rc o1 o2) /\ Fst_then_snd? (rc ob ol) /\ 
                     distinct_ops o1 o2 /\ distinct_ops o1 ob /\ distinct_ops o1 ol /\ distinct_ops o2 ob /\ distinct_ops o2 ol /\ distinct_ops ob ol /\ 
                     eq (merge (do l ol) (do (do a ol) o1) (do (do b ol) o2)) (do (do (do c ol) o1) o2) /\
                     eq (merge l (do a o1) (do b o2)) (do (do c o1) o2) /\
                     eq (merge l (do a ol) (do b ob)) (do (do c ob) ol)) //***EXTRA***
-          (ensures eq (merge (do l ol) (do (do a ol) o1) (do (do (do b ob) ol) o2)) (do (do (do (do c ob) ol) o1) o2))
+          (ensures eq (merge (do l ol) (do (do a ol) o1) (do (do (do b ob) ol) o2)) (do (do (do (do c ob) ol) o1) o2)) = ()
 
-val rc_inter_base_left (l a b c:concrete_st) (o1 o2 ob ol:op_t) 
+let rc_inter_base_left (l a b c:concrete_st) (o1 o2 ob ol:op_t) 
   : Lemma (requires Fst_then_snd? (rc o1 o2) /\ Fst_then_snd? (rc ob ol) /\ 
                     distinct_ops o1 o2 /\ distinct_ops o1 ob /\ distinct_ops o1 ol /\ distinct_ops o2 ob /\ distinct_ops o2 ol /\ distinct_ops ob ol /\ 
                     eq (merge (do l ol) (do (do a ol) o1) (do (do b ol) o2)) (do (do (do c ol) o1) o2) /\
                     eq (merge l (do a o1) (do b o2)) (do (do c o1) o2) /\
                     eq (merge l (do a ob) (do b ol)) (do (do c ob) ol)) //***EXTRA***
-          (ensures eq (merge (do l ol) (do (do (do a ob) ol) o1) (do (do b ol) o2)) (do (do (do (do c ob) ol) o1) o2))
+          (ensures eq (merge (do l ol) (do (do (do a ob) ol) o1) (do (do b ol) o2)) (do (do (do (do c ob) ol) o1) o2)) = ()
           
-val rc_inter_right (l a b c:concrete_st) (o1 o2 ob ol o:op_t)
+let rc_inter_right (l a b c:concrete_st) (o1 o2 ob ol o:op_t)
   : Lemma (requires Fst_then_snd? (rc o1 o2) /\ Fst_then_snd? (rc ob ol) /\ 
                     distinct_ops o1 o2 /\ distinct_ops o1 ob /\ distinct_ops o1 ol /\ distinct_ops o1 o /\ distinct_ops o2 ob /\ 
                     distinct_ops o2 ol /\ distinct_ops o2 o /\ distinct_ops ob ol /\ distinct_ops ob o /\ distinct_ops ol o /\
                     get_rid o <> get_rid ol (*o,ol must be concurrent*) /\
                     ((~ (commutes_with o ob)) \/ Fst_then_snd? (rc o ol)) /\
                     eq (merge (do l ol) (do (do a ol) o1) (do (do (do b ob) ol) o2)) (do (do (do (do c ob) ol) o1) o2))
-      (ensures eq (merge (do l ol) (do (do a ol) o1) (do (do (do (do b o) ob) ol) o2)) (do (do (do (do (do c o) ob) ol) o1) o2))
+      (ensures eq (merge (do l ol) (do (do a ol) o1) (do (do (do (do b o) ob) ol) o2)) (do (do (do (do (do c o) ob) ol) o1) o2)) = ()
 
-val rc_inter_left (l a b c:concrete_st) (o1 o2 ob ol o:op_t)
+let rc_inter_left (l a b c:concrete_st) (o1 o2 ob ol o:op_t)
   : Lemma (requires Fst_then_snd? (rc o1 o2) /\ Fst_then_snd? (rc ob ol) /\ 
                     distinct_ops o1 o2 /\ distinct_ops o1 ob /\ distinct_ops o1 ol /\ distinct_ops o1 o /\ distinct_ops o2 ob /\ 
                     distinct_ops o2 ol /\ distinct_ops o2 o /\ distinct_ops ob ol /\ distinct_ops ob o /\ distinct_ops ol o /\
                     get_rid o <> get_rid ol (*o,ol must be concurrent*) /\
                     ((~ (commutes_with o ob)) \/ Fst_then_snd? (rc o ol)) /\
                     eq (merge (do l ol) (do (do (do a ob) ol) o1) (do (do b ol) o2)) (do (do (do (do c ob) ol) o1) o2))
-      (ensures eq (merge (do l ol) (do (do (do (do a o) ob) ol) o1) (do (do b ol) o2)) (do (do (do (do (do c o) ob) ol) o1) o2))
+      (ensures eq (merge (do l ol) (do (do (do (do a o) ob) ol) o1) (do (do b ol) o2)) (do (do (do (do (do c o) ob) ol) o1) o2)) = ()
 
 // In general, the events ol,oi, below should be such that these exists o, (rc o ol), (rc o oi)
-val rc_inter_lca (l a b c:concrete_st) (o1 o2 ol oi:op_t)
+let rc_inter_lca (l a b c:concrete_st) (o1 o2 ol oi:op_t)
   : Lemma (requires distinct_ops o1 o2 /\ Fst_then_snd? (rc o1 o2) /\ 
                     (exists o. Fst_then_snd? (rc o ol)) /\ 
                     (exists o. Fst_then_snd? (rc o oi)) /\ 
                     eq (merge (do l oi) (do (do a oi) o1) (do (do b oi) o2)) (do (do (do c oi) o1) o2) /\
                     eq (merge (do l ol) (do (do a ol) o1) (do (do b ol) o2)) (do (do (do c ol) o1) o2))
-    (ensures eq (merge (do (do l oi) ol) (do (do (do a oi) ol) o1) (do (do (do b oi) ol) o2)) (do (do (do (do c oi) ol) o1) o2))
+    (ensures eq (merge (do (do l oi) ol) (do (do (do a oi) ol) o1) (do (do (do b oi) ol) o2)) (do (do (do (do c oi) ol) o1) o2)) = ()
 
 (*One op*)
 ///////////////
-val one_op_ind_right (l a b c:concrete_st) (o2 o2':op_t)
+let one_op_ind_right (l a b c:concrete_st) (o2 o2':op_t)
    : Lemma (requires eq (merge l a (do b o2)) (do (merge l a b) o2))
-           (ensures eq (merge l a (do (do b o2') o2)) (do (merge l a (do b o2')) o2))
+           (ensures eq (merge l a (do (do b o2') o2)) (do (merge l a (do b o2')) o2)) = ()
 
-val one_op_ind_left (l a b c:concrete_st) (o1 o1':op_t)
+let one_op_ind_left (l a b c:concrete_st) (o1 o1':op_t)
    : Lemma (requires eq (merge l (do a o1) b) (do (merge l a b) o1))
-           (ensures eq (merge l (do (do a o1') o1) b) (do (merge l (do a o1') b) o1))
+           (ensures eq (merge l (do (do a o1') o1) b) (do (merge l (do a o1') b) o1)) = ()
            
-val one_op_ind_lca (l:concrete_st) (o2 o:op_t)
+let one_op_ind_lca (l:concrete_st) (o2 o:op_t)
   : Lemma (requires eq (merge l l (do l o2)) (do l o2))
-          (ensures eq (merge (do l o) (do l o) (do (do l o) o2)) (do (do l o) o2)) 
+          (ensures eq (merge (do l o) (do l o) (do (do l o) o2)) (do (do l o) o2)) = () 
 
-val one_op_base (o2:op_t)
-  : Lemma (ensures eq (merge init_st init_st (do init_st o2)) (do init_st o2))
+let one_op_base (o2:op_t)
+  : Lemma (ensures eq (merge init_st init_st (do init_st o2)) (do init_st o2)) = ()
 
-val one_op_inter_base_right (l a b c:concrete_st) (o2 ob ol:op_t) 
+let one_op_inter_base_right (l a b c:concrete_st) (o2 ob ol:op_t) 
   : Lemma (requires Fst_then_snd? (rc ob ol) /\
                     distinct_ops o2 ob /\ distinct_ops o2 ol /\ distinct_ops ob ol /\
                     eq (merge (do l ol) (do a ol) (do (do b ol) o2)) (do (do c ol) o2) /\
                     eq (merge l a (do b o2)) (do c o2) /\
                     eq (merge l (do a ol) (do b ob)) (do (do c ob) ol)) //***EXTRA***
-          (ensures eq (merge (do l ol) (do a ol) (do (do (do b ob) ol) o2)) (do (do (do c ob) ol) o2))
+          (ensures eq (merge (do l ol) (do a ol) (do (do (do b ob) ol) o2)) (do (do (do c ob) ol) o2)) = ()
 
-val one_op_inter_base_left (l a b c:concrete_st) (o2 ob ol:op_t) 
+let one_op_inter_base_left (l a b c:concrete_st) (o2 ob ol:op_t) 
   : Lemma (requires Fst_then_snd? (rc ob ol) /\
                     distinct_ops o2 ob /\ distinct_ops o2 ol /\ distinct_ops ob ol /\
                     eq (merge (do l ol) (do a ol) (do (do b ol) o2)) (do (do c ol) o2) /\
@@ -185,82 +210,82 @@ val one_op_inter_base_left (l a b c:concrete_st) (o2 ob ol:op_t)
                     eq (merge l a (do b o2)) (do c o2) /\
                     eq (merge l (do a ol) (do b ob)) (do (do c ob) ol) /\ //***EXTRA***
                     eq (merge l (do (do a ob) ol) (do b ol)) (do (do c ob) ol)) //***EXTRA***
-          (ensures eq (merge (do l ol) (do (do a ob) ol) (do (do b ol) o2)) (do (do (do c ob) ol) o2))
+          (ensures eq (merge (do l ol) (do (do a ob) ol) (do (do b ol) o2)) (do (do (do c ob) ol) o2)) = ()
 
-val one_op_inter_right (l a b c:concrete_st) (o2 ob ol o:op_t) 
+let one_op_inter_right (l a b c:concrete_st) (o2 ob ol o:op_t) 
   : Lemma (requires Fst_then_snd? (rc ob ol) /\
                     distinct_ops o ob /\ distinct_ops o ol /\ distinct_ops o ol /\ distinct_ops ob ol /\ distinct_ops ob o2 /\ distinct_ops o2 ol /\
                     get_rid o <> get_rid ol (*o,ol must be concurrent*) /\
                     ((~ (commutes_with o ob)) \/ Fst_then_snd? (rc o ol)) /\
                     eq (merge (do l ol) (do a ol) (do (do (do b ob) ol) o2)) (do (do (do c ob) ol) o2))
-          (ensures eq (merge (do l ol) (do a ol) (do (do (do (do b o) ob) ol) o2)) (do (do (do (do c o) ob) ol) o2))
+          (ensures eq (merge (do l ol) (do a ol) (do (do (do (do b o) ob) ol) o2)) (do (do (do (do c o) ob) ol) o2)) = ()
           
-val one_op_inter_left (l a b c:concrete_st) (o2 ob ol o:op_t) 
+let one_op_inter_left (l a b c:concrete_st) (o2 ob ol o:op_t) 
   : Lemma (requires Fst_then_snd? (rc ob ol) /\
                     distinct_ops o ob /\ distinct_ops o ol /\ distinct_ops o ol /\ distinct_ops ob ol /\ distinct_ops ob o2 /\ distinct_ops o2 ol /\
                     get_rid o <> get_rid ol (*o,ol must be concurrent*) /\
                     ((~ (commutes_with o ob)) \/ Fst_then_snd? (rc o ol)) /\
                     eq (merge (do l ol) (do (do a ob) ol) (do (do b ol) o2)) (do (do (do c ob) ol) o2))
-          (ensures eq (merge (do l ol) (do (do (do a o) ob) ol) (do (do b ol) o2)) (do (do (do (do c o) ob) ol) o2))
+          (ensures eq (merge (do l ol) (do (do (do a o) ob) ol) (do (do b ol) o2)) (do (do (do (do c o) ob) ol) o2)) = ()
 
 // In general, the events o',o_n, below should be such that these exists o, (rc o o')
-val one_op_inter_lca (l a b c:concrete_st) (o2 ol oi:op_t)
+let one_op_inter_lca (l a b c:concrete_st) (o2 ol oi:op_t)
   : Lemma (requires (exists o. Fst_then_snd? (rc o ol)) /\ 
                     (exists o. Fst_then_snd? (rc o oi)) /\ 
                     eq (merge (do l oi) (do a oi) (do (do b oi) o2)) (do (do c oi) o2) /\
                     eq (merge (do l ol) (do a ol) (do (do b ol) o2)) (do (do c ol) o2))
-          (ensures eq (merge (do (do l oi) ol) (do (do a oi) ol) (do (do (do b oi) ol) o2)) (do (do (do c oi) ol) o2))
+          (ensures eq (merge (do (do l oi) ol) (do (do a oi) ol) (do (do (do b oi) ol) o2)) (do (do (do c oi) ol) o2)) = ()
 
 (*Zero op *)
 ///////////////
 // because we proved that e_i^l rcp eb is not possible.
 //e_i^l vis eb is not possible
 // so either eb rcp e_i^l or eb rct e_i^l is possible
-val zero_op_inter_base_right (l a b c:concrete_st) (ob ol:op_t) 
+let zero_op_inter_base_right (l a b c:concrete_st) (ob ol:op_t) 
   : Lemma (requires Fst_then_snd? (rc ob ol) /\ distinct_ops ob ol /\ 
                     eq (merge (do l ol) (do a ol) (do b ol)) (do c ol) /\
                     eq (merge l a b) c /\
                     eq (merge l (do a ol) (do b ob)) (do (do c ob) ol)) //***EXTRA***
-          (ensures eq (merge (do l ol) (do a ol) (do (do b ob) ol)) (do (do c ob) ol)) 
+          (ensures eq (merge (do l ol) (do a ol) (do (do b ob) ol)) (do (do c ob) ol)) = () 
 
-val zero_op_inter_base_left (l a b c:concrete_st) (ob ol:op_t) 
+let zero_op_inter_base_left (l a b c:concrete_st) (ob ol:op_t) 
   : Lemma (requires Fst_then_snd? (rc ob ol) /\ distinct_ops ob ol /\ 
                     eq (merge (do l ol) (do a ol) (do b ol)) (do c ol) /\
                     eq (merge l a b) c /\
                     eq (merge l (do a ob) (do b ol)) (do (do c ob) ol)) //***EXTRA***
-          (ensures eq (merge (do l ol) (do (do a ob) ol) (do b ol) ) (do (do c ob) ol)) 
+          (ensures eq (merge (do l ol) (do (do a ob) ol) (do b ol) ) (do (do c ob) ol)) = () 
 
-val zero_op_inter_right (l a b c:concrete_st) (ob ol o:op_t)
+let zero_op_inter_right (l a b c:concrete_st) (ob ol o:op_t)
   : Lemma (requires Fst_then_snd? (rc ob ol) /\ distinct_ops ob ol /\ 
                     get_rid o <> get_rid ol (*o,ol must be concurrent*) /\
                     ((~ (commutes_with o ob)) \/ Fst_then_snd? (rc o ol)) /\
                     eq (merge (do l ol) (do a ol) (do (do b ob) ol)) (do (do c ob) ol))
-          (ensures eq (merge (do l ol) (do a ol) (do (do (do b o) ob) ol)) (do (do (do c o) ob) ol)) 
+          (ensures eq (merge (do l ol) (do a ol) (do (do (do b o) ob) ol)) (do (do (do c o) ob) ol)) = ()
 
-val zero_op_inter_left (l a b c:concrete_st) (ob ol o:op_t)
+let zero_op_inter_left (l a b c:concrete_st) (ob ol o:op_t)
   : Lemma (requires Fst_then_snd? (rc ob ol) /\ distinct_ops ob ol /\ 
                     get_rid o <> get_rid ol (*o,ol must be concurrent*) /\
                     ((~ (commutes_with o ob)) \/ Fst_then_snd? (rc o ol)) /\
                     eq (merge (do l ol) (do (do a ob) ol) (do b ol)) (do (do c ob) ol))
-          (ensures eq (merge (do l ol) (do (do (do a o) ob) ol) (do b ol)) (do (do (do c o) ob) ol)) 
+          (ensures eq (merge (do l ol) (do (do (do a o) ob) ol) (do b ol)) (do (do (do c o) ob) ol)) = ()
 
 // In general, the event "o" below should be such that these exists o', (rc o' o)
-val zero_op_inter_lca_v1 (l a b c:concrete_st) (ol:op_t)
+let zero_op_inter_lca_v1 (l a b c:concrete_st) (ol:op_t)
   : Lemma (requires (exists o'. Fst_then_snd? (rc o' ol)) /\ eq (merge l a b) c)
-          (ensures eq (merge (do l ol) (do a ol) (do b ol)) (do c ol))
+          (ensures eq (merge (do l ol) (do a ol) (do b ol)) (do c ol)) = ()
 
 // In general, the events o',o_n, below should be such that these exists o, (rc o o')
-val zero_op_inter_lca_v2 (l a b c:concrete_st) (ol oi:op_t)
+let zero_op_inter_lca_v2 (l a b c:concrete_st) (ol oi:op_t)
   : Lemma (requires (exists o. Fst_then_snd? (rc o ol)) /\ 
                     (exists o. Fst_then_snd? (rc o oi)) /\
                     eq (merge (do l oi) (do a oi) (do b oi)) (do c oi)  /\
                     eq (merge (do l ol) (do a ol) (do b ol)) (do c ol))
-          (ensures eq (merge (do (do l oi) ol) (do (do a oi) ol) (do (do b oi) ol)) (do (do c oi) ol))
+          (ensures eq (merge (do (do l oi) ol) (do (do a oi) ol) (do (do b oi) ol)) (do (do c oi) ol)) = ()
 
 (* 2 op Comm  *)
 ///////////////////
 
-val comm_ind_right (l a b c:concrete_st) (o1 o2 o2':op_t)
+let comm_ind_right (l a b c:concrete_st) (o1 o2 o2':op_t)
   : Lemma (requires Either? (rc o1 o2) /\ 
                     distinct_ops o1 o2 /\ distinct_ops o1 o2' /\ distinct_ops o2 o2' /\
                     eq (merge l (do a o1) (do b o2)) (do (do (merge l a b) o2) o1) /\
@@ -269,9 +294,9 @@ val comm_ind_right (l a b c:concrete_st) (o1 o2 o2':op_t)
                     ~ (Fst_then_snd? (rc o1 o2')) /\
                     ~ (exists o3 b'. eq (do (do b o2') o2) (do b' o3) /\ distinct_ops o1 o3 /\ Fst_then_snd? (rc o1 o3)) /\
                     ~ (exists o3 b'. eq (do b o2) (do b' o3) /\ distinct_ops o1 o3 /\ Fst_then_snd? (rc o1 o3)))                    
-          (ensures eq (merge l (do a o1) (do (do b o2') o2)) (do (do (merge l a (do b o2')) o2) o1))
+          (ensures eq (merge l (do a o1) (do (do b o2') o2)) (do (do (merge l a (do b o2')) o2) o1)) = ()
 
-val comm_ind_left (l a b c:concrete_st) (o1 o2 o1':op_t)
+let comm_ind_left (l a b c:concrete_st) (o1 o2 o1':op_t)
   : Lemma (requires Either? (rc o1 o2) /\ 
                     distinct_ops o1 o2 /\ distinct_ops o1 o1' /\ distinct_ops o2 o1' /\
                     eq (merge l (do a o1) (do b o2)) (do (do (merge l a b) o2) o1) /\
@@ -280,37 +305,37 @@ val comm_ind_left (l a b c:concrete_st) (o1 o2 o1':op_t)
                     ~ (Fst_then_snd? (rc o2 o1')) /\
                     ~ (exists o3 b'. eq (do (do b o1') o2) (do b' o3) /\ distinct_ops o1 o3 /\ Fst_then_snd? (rc o1 o3)) /\
                     ~ (exists o3 b'. eq (do b o2) (do b' o3) /\ distinct_ops o1 o3 /\ Fst_then_snd? (rc o1 o3)))                    
-          (ensures eq (merge l (do (do a o1') o1) (do b o2)) (do (do (merge l (do a o1') b) o2) o1))
+          (ensures eq (merge l (do (do a o1') o1) (do b o2)) (do (do (merge l (do a o1') b) o2) o1)) = ()
 
-val comm_ind_lca (l:concrete_st) (o1 o2 ol:op_t)
+let comm_ind_lca (l:concrete_st) (o1 o2 ol:op_t)
   : Lemma (requires Either? (rc o1 o2) /\ 
                     distinct_ops o1 o2 /\ distinct_ops o1 ol /\ distinct_ops o2 ol /\
                     eq (merge l (do l o1) (do l o2)) (do (do l o2) o1))
-          (ensures eq (merge (do l ol) (do (do l ol) o1) (do (do l ol) o2)) (do (do (do l ol) o2) o1))
+          (ensures eq (merge (do l ol) (do (do l ol) o1) (do (do l ol) o2)) (do (do (do l ol) o2) o1)) = ()
 
-val comm_base (o1 o2:op_t)
+let comm_base (o1 o2:op_t)
   : Lemma (requires Either? (rc o1 o2) /\ distinct_ops o1 o2)
-          (ensures eq (merge init_st (do init_st o1) (do init_st o2)) (do (do init_st o1) o2))
+          (ensures eq (merge init_st (do init_st o1) (do init_st o2)) (do (do init_st o1) o2)) = ()
 
-val comm_inter_base_right (l a b c:concrete_st) (o1 o2 ob ol:op_t) 
+let comm_inter_base_right (l a b c:concrete_st) (o1 o2 ob ol:op_t) 
   : Lemma (requires Either? (rc o1 o2) /\ Fst_then_snd? (rc ob ol) /\ 
                     distinct_ops o1 o2 /\ distinct_ops o1 ob /\ distinct_ops o1 ol /\ distinct_ops o2 ob /\ distinct_ops o2 ol /\ distinct_ops ob ol /\
                     eq (merge (do l ol) (do (do a ol) o1) (do (do b ol) o2)) (do (do (do c ol) o1) o2) /\ 
                     eq (merge l (do a o1) (do b o2)) (do (do c o1) o2) /\
                     eq (merge l (do a o1) (do (do b ob) o2)) (do (do (merge l a (do b ob)) o1) o2) /\ //comes from comm_ind_right
                     eq (merge (do l ol) (do a ol) (do (do b ob) ol)) (do (do c ob) ol)) //comes from intermediate_base_zero_op
-          (ensures eq (merge (do l ol) (do (do a ol) o1) (do (do (do b ob) ol) o2)) (do (do (do (do c ob) ol) o1) o2))
+          (ensures eq (merge (do l ol) (do (do a ol) o1) (do (do (do b ob) ol) o2)) (do (do (do (do c ob) ol) o1) o2)) = ()
 
-val comm_inter_base_left (l a b c:concrete_st) (o1 o2 ob ol:op_t) 
+let comm_inter_base_left (l a b c:concrete_st) (o1 o2 ob ol:op_t) 
   : Lemma (requires Either? (rc o1 o2) /\ Fst_then_snd? (rc ob ol) /\ 
                     distinct_ops o1 o2 /\ distinct_ops o1 ob /\ distinct_ops o1 ol /\ distinct_ops o2 ob /\ distinct_ops o2 ol /\ distinct_ops ob ol /\
                     eq (merge (do l ol) (do (do a ol) o1) (do (do b ol) o2)) (do (do (do c ol) o1) o2) /\ 
                     eq (merge l (do a o1) (do b o2)) (do (do c o1) o2) /\
                     eq (merge l (do (do a ob) o1) (do b o2)) (do (do (merge l (do a ob) b) o1) o2) /\ //comes from comm_ind_left
                     eq (merge (do l ol) (do (do a ob) ol) (do b ol)) (do (do c ob) ol)) //comes from intermediate_base_zero_op
-          (ensures eq (merge (do l ol) (do (do (do a ob) ol) o1) (do (do b ol) o2)) (do (do (do (do c ob) ol) o1) o2))
+          (ensures eq (merge (do l ol) (do (do (do a ob) ol) o1) (do (do b ol) o2)) (do (do (do (do c ob) ol) o1) o2)) = ()
 
-val comm_inter_right (l a b c:concrete_st) (o1 o2 ob ol o:op_t)
+let comm_inter_right (l a b c:concrete_st) (o1 o2 ob ol o:op_t)
   : Lemma (requires Either? (rc o1 o2) /\ Fst_then_snd? (rc ob ol) /\ 
                     distinct_ops o1 o2 /\ distinct_ops o1 ob /\ distinct_ops o1 ol /\ distinct_ops o1 o /\ distinct_ops o2 ob /\ 
                     distinct_ops o2 ol /\ distinct_ops o2 o /\ distinct_ops ob ol /\ distinct_ops ob o /\ distinct_ops ol o /\
@@ -318,9 +343,9 @@ val comm_inter_right (l a b c:concrete_st) (o1 o2 ob ol o:op_t)
                     //Either? (rc o ol) /\ 
                     ((~ (commutes_with o ob)) \/ Fst_then_snd? (rc o ol)) /\
                     eq (merge (do l ol) (do (do a ol) o1) (do (do (do b ob) ol) o2)) (do (do (do (do c ob) ol) o1) o2))
-          (ensures eq (merge (do l ol) (do (do a ol) o1) (do (do (do (do b o) ob) ol) o2)) (do (do (do (do (do c o) ob) ol) o1) o2))
+          (ensures eq (merge (do l ol) (do (do a ol) o1) (do (do (do (do b o) ob) ol) o2)) (do (do (do (do (do c o) ob) ol) o1) o2)) = ()
 
-val comm_inter_left (l a b c:concrete_st) (o1 o2 ob ol o:op_t)
+let comm_inter_left (l a b c:concrete_st) (o1 o2 ob ol o:op_t)
   : Lemma (requires Either? (rc o1 o2) /\ Fst_then_snd? (rc ob ol) /\ 
                     distinct_ops o1 o2 /\ distinct_ops o1 ob /\ distinct_ops o1 ol /\ distinct_ops o1 o /\ distinct_ops o2 ob /\ 
                     distinct_ops o2 ol /\ distinct_ops o2 o /\ distinct_ops ob ol /\ distinct_ops ob o /\ distinct_ops ol o /\
@@ -328,38 +353,40 @@ val comm_inter_left (l a b c:concrete_st) (o1 o2 ob ol o:op_t)
                     //Either? (rc o ol) /\ 
                     ((~ (commutes_with o ob)) \/ Fst_then_snd? (rc o ol)) /\
                     eq (merge (do l ol) (do (do (do a ob) ol) o1) (do (do b ol) o2)) (do (do (do (do c ob) ol) o1) o2))
-          (ensures eq (merge (do l ol) (do (do (do (do a o) ob) ol) o1) (do (do b ol) o2)) (do (do (do (do (do c o) ob) ol) o1) o2))
+          (ensures eq (merge (do l ol) (do (do (do (do a o) ob) ol) o1) (do (do b ol) o2)) (do (do (do (do (do c o) ob) ol) o1) o2)) = ()
 
-val comm_inter_lca (l a b c:concrete_st) (o1 o2 ol:op_t)
+let comm_inter_lca (l a b c:concrete_st) (o1 o2 ol:op_t)
   : Lemma (requires Either? (rc o1 o2) /\ 
                     distinct_ops o1 o2 /\ distinct_ops o1 ol /\ distinct_ops ol o2 /\
                     (exists o'. Fst_then_snd? (rc o' ol)) /\
                     eq (merge l (do a o1) (do b o2)) (do (do c o1) o2))
-          (ensures eq (merge (do l ol) (do (do a ol) o1) (do (do b ol) o2)) (do (do (do c ol) o1) o2))
+          (ensures eq (merge (do l ol) (do (do a ol) o1) (do (do b ol) o2)) (do (do (do c ol) o1) o2)) = ()
 
 ////////////////////////////////////////////////////////////////
 //// Sequential implementation //////
 
 // the concrete state 
-val concrete_st_s : Type0
+let concrete_st_s = bool
 
 // init state 
-val init_st_s : concrete_st_s
+let init_st_s = false
 
 // apply an operation to a state 
-val do_s (st_s:concrete_st_s) (_:op_t) : concrete_st_s
+let do_s (st_s:concrete_st_s) (o:op_t) =
+  if Enable? (snd (snd o)) then true else false
 
 // equivalence relation between the concrete states of sequential type and MRDT
-val eq_sm (st_s:concrete_st_s) (st:concrete_st) : Type0
+let eq_sm (st_s:concrete_st_s) (st:concrete_st) =
+  st_s <==> (exists rid. snd (sel st rid) = true)
 
 // initial states are equivalent
-val initial_eq (_:unit)
-  : Lemma (ensures eq_sm init_st_s init_st)
+let initial_eq (_:unit)
+  : Lemma (ensures eq_sm init_st_s init_st) = ()
 
 // equivalence between states of sequential type and MRDT at every operation
-val do_eq (st_s:concrete_st_s) (st:concrete_st) (op:op_t)
+let do_eq (st_s:concrete_st_s) (st:concrete_st) (op:op_t)
   : Lemma (requires eq_sm st_s st)
-          (ensures eq_sm (do_s st_s op) (do st op))
+          (ensures eq_sm (do_s st_s op) (do st op)) = ()
 
 ////////////////////////////////////////////////////////////////
 
@@ -367,33 +394,34 @@ val do_eq (st_s:concrete_st_s) (st:concrete_st) (op:op_t)
 ////Equivalence of  MRDT & Sequential implementation  //////
 
 // the concrete state 
-(*val concrete_st_s : Type0
+(*let concrete_st_s = bool
 
 // init state 
-val init_st_s : concrete_st_s
+let init_st_s = false
 
 // apply an operation to a state 
-val do_s (st_s:concrete_st_s) (_:op_t) : concrete_st_s
+let do_s (st_s:concrete_st_s) (o:op_t) = 
+  if Enable? (snd (snd o)) then true else false
 
 //query type
-val query_t : eqtype
+type query_t = unit //is the element present?
 
 //ret type
-val ret_t : Type0
+type ret_t1 = prop
 
 //query return value - MRDT
-val query_m (s:concrete_st) (q:query_t) : ret_t
+let query_m1 (s:concrete_st) (q:query_t) : ret_t1 = exists rid. M.contains s rid /\ snd (sel s rid) == true
 
 //query return value - Seq impl
-val query_s (s:concrete_st_s) (q:query_t) : ret_t
+let query_s1 (s:concrete_st_s) (q:query_t) : ret_t1 = s
 
 // initial states are equivalent
-val initial_eq (q:query_t)
-  : Lemma (ensures query_s init_st_s q == query_m init_st q)
+let initial_eq1 (q:query_t)
+  : Lemma (ensures query_s1 init_st_s q == query_m1 init_st q) = ()
 
 //equivalence between states of sequential type and MRDT at every operation
-val do_eq (st_s:concrete_st_s) (st:concrete_st) (op:op_t) (q:query_t)
-  : Lemma (requires query_s st_s q == query_m st q)
-          (ensures query_s (do_s st_s op) q == query_m (do st op) q)*)
+let do_eq1 (st_s:concrete_st_s) (st:concrete_st) (op:op_t) (q:query_t)
+  : Lemma (requires query_s1 st_s q == query_m1 st q)
+          (ensures query_s1 (do_s st_s op) q == query_m1 (do st op) q) = ()*)
          
 ////////////////////////////////////////////////////////////////
