mrdts-new/Remove-wins_set/App.fst
@@ -1,183 +1,197 @@
 module App
 
-open FStar.Seq
+module S = Set_extended
+
+#set-options "--query_stats"
 
 // the concrete state type
-val concrete_st : Type0
+type concrete_st = s:S.t (nat * nat){forall e. S.mem e s ==> ((snd e = 1) \/ (snd e = 2))} //(nat & nat)
 
 // init state
-val init_st : concrete_st
+let init_st : concrete_st = S.add (0,1) (S.add (0,2) S.empty)
 
 // equivalence between 2 concrete states
-val eq (a b:concrete_st) : Type0
+let eq (a b:concrete_st) =
+  S.equal a b
 
-val symmetric (a b:concrete_st) 
+let symmetric (a b:concrete_st) 
   : Lemma (requires eq a b)
-          (ensures eq b a)
+          (ensures eq b a) = ()
 
-val transitive (a b c:concrete_st)
+let transitive (a b c:concrete_st)
   : Lemma (requires eq a b /\ eq b c)
-          (ensures eq a c)
+          (ensures eq a c) = ()
 
-val eq_is_equiv (a b:concrete_st)
+let eq_is_equiv (a b:concrete_st)
   : Lemma (requires a == b)
-          (ensures eq a b)
+          (ensures eq a b) = ()
 
 // operation type
-val app_op_t : eqtype 
-
-type op_t = pos (*timestamp*) & (nat (*replica ID*) & app_op_t)
-
-let get_rid (_,(rid,_)) = rid
-
-let distinct_ops (op1 op2:op_t) = fst op1 =!= fst op2
-
-type log = seq op_t
+type app_op_t:eqtype =
+  |Add1
+  |Rem1
+  |Add2
+  |Rem2
 
 // apply an operation to a state
-val do (s:concrete_st) (o:op_t) : concrete_st
-
-let commutes_with (o1 o2:op_t) =
-  forall s. eq (do (do s o1) o2) (do (do s o2) o1)
-
-// applying a log of operations to a concrete state
-let rec apply_log (x:concrete_st) (l:log) : Tot concrete_st (decreases length l) =
-  match length l with
-  |0 -> x
-  |_ -> apply_log (do x (head l)) (tail l)  
-  
-//conflict resolution type
-type rc_res =
-  |Fst_then_snd //o1 -> o2
-  |Snd_then_fst //o2 -> o1
-  |Either
+let do (s:concrete_st) (o:op_t) : concrete_st =
+ match o with
+  |(_, (rid, Add1)) -> S.filter s (fun e -> snd e <> 1)
+  |(ts, (rid, Rem1)) -> S.add (ts, 1) s
+  |(_, (rid, Add2)) -> S.filter s (fun e -> snd e <> 2)
+  |(ts, (rid, Rem2)) -> S.add (ts, 2) s
 
 //conflict resolution
-val rc (o1 o2:op_t) : rc_res
+let rc (o1 o2:op_t) =
+  match snd (snd o1), snd (snd o2) with
+  |Add1, Rem1 |Add2, Rem2 -> Fst_then_snd
+  |Rem1, Add1 | Rem2, Add2 -> Snd_then_fst
+  |_ -> Either
 
 // concrete merge operation
-val merge (l a b:concrete_st) : concrete_st
+let merge (l a b:concrete_st) : concrete_st =
+  let da = S.difference a l in
+  let db = S.difference b l in
+  let i_ab = S.intersection a b in
+  let i_lab = S.intersection l i_ab in
+  S.union i_lab (S.union da db)
 
 /////////////////////////////////////////////////////////////////////////////
 
-val rc_non_comm (o1 o2:op_t)
+let rc_non_comm_help1 (o1 o2:op_t)
   : Lemma (requires distinct_ops o1 o2)
-          (ensures Either? (rc o1 o2) <==> commutes_with o1 o2)
+          (ensures ((Add1? (snd (snd o1)) /\ Rem1? (snd (snd o2))) \/ (Rem1? (snd (snd o1)) /\ Add1? (snd (snd o2))))
+                           ==> ~ (eq (do (do init_st o1) o2) (do (do init_st o2) o1))) = ()
+         
+let rc_non_comm_help2 (o1 o2:op_t)
+  : Lemma (requires distinct_ops o1 o2)
+          (ensures ((Add2? (snd (snd o1)) /\ Rem2? (snd (snd o2))) \/ (Rem2? (snd (snd o1)) /\ Add2? (snd (snd o2))))
+                           ==> ~ (eq (do (do init_st o1) o2) (do (do init_st o2) o1))) = ()
+          
+let rc_non_comm (o1 o2:op_t)
+  : Lemma (requires distinct_ops o1 o2)
+          (ensures Either? (rc o1 o2) <==> commutes_with o1 o2) = 
+  rc_non_comm_help1 o1 o2;
+  rc_non_comm_help2 o1 o2
 
-val no_rc_chain (o1 o2 o3:op_t)
+let no_rc_chain (o1 o2 o3:op_t)
   : Lemma (requires distinct_ops o1 o2 /\ distinct_ops o2 o3)
-          (ensures ~ (Fst_then_snd? (rc o1 o2) /\ Fst_then_snd? (rc o2 o3)))
+          (ensures ~ (Fst_then_snd? (rc o1 o2) /\ Fst_then_snd? (rc o2 o3))) = ()
 
-val cond_comm_base (s:concrete_st) (o1 o2:op_t) (o3:op_t{distinct_ops o1 o2 /\ distinct_ops o1 o3 /\ distinct_ops o2 o3})
-    : (b:bool{(Fst_then_snd? (rc o1 o2) /\ ~ (Either? (rc o2 o3))) ==> eq (do (do (do s o1) o2) o3) (do (do (do s o2) o1) o3)})
+let cond_comm_base (s:concrete_st) (o1 o2:op_t) (o3:op_t{distinct_ops o1 o2 /\ distinct_ops o1 o3 /\ distinct_ops o2 o3})
+    : (b:bool{(Fst_then_snd? (rc o1 o2) /\ ~ (Either? (rc o2 o3))) ==> eq (do (do (do s o1) o2) o3) (do (do (do s o2) o1) o3)}) = 
+    if ((Add1? (snd (snd o3)) && (Add1? (snd (snd o1)) || Rem1? (snd (snd o1)))) || 
+      (Add2? (snd (snd o3)) && (Add2? (snd (snd o1)) || Rem2? (snd (snd o1))))) then true else false
 
-val cond_comm_ind (s:concrete_st) (o1 o2 o3 o:op_t) (l:seq op_t)
+let cond_comm_ind (s:concrete_st) (o1 o2 o3 o:op_t) (l:seq op_t)
   : Lemma (requires distinct_ops o1 o2 /\ distinct_ops o1 o3 /\ distinct_ops o2 o3 /\ cond_comm_base s o1 o2 o3 /\
                     eq (do (apply_log (do (do s o1) o2) l) o3) (do (apply_log (do (do s o2) o1) l) o3))
-          (ensures eq (do (do (apply_log (do (do s o1) o2) l) o) o3) (do (do (apply_log (do (do s o2) o1) l) o) o3))
-                  
-////////////////////////////////////////////////////////////////////////////
+          (ensures eq (do (do (apply_log (do (do s o1) o2) l) o) o3) (do (do (apply_log (do (do s o2) o1) l) o) o3)) = ()
+                   
+/////////////////////////////////////////////////////////////////////////////
+// Merge commutativity
+let merge_comm (l a b:concrete_st)
+   : Lemma (ensures (eq (merge l a b) (merge l b a))) = ()
 
-val merge_comm (l a b:concrete_st)
-  : Lemma (ensures (eq (merge l a b) (merge l b a)))
-                       
-val merge_idem (s:concrete_st)
-  : Lemma (ensures eq (merge s s s) s)
+// Merge idempotence
+let merge_idem (s:concrete_st)
+   : Lemma (ensures eq (merge s s s) s) = ()
 
+#push-options "--z3rlimit 100 --max_ifuel 3"
 (*Two OP RC*)
 //////////////// 
-val rc_ind_right (l a b:concrete_st) (o1 o2 o2':op_t)
+let rc_ind_right (l a b:concrete_st) (o1 o2 o2':op_t)
   : Lemma (requires Fst_then_snd? (rc o1 o2) /\
                     distinct_ops o1 o2 /\ distinct_ops o1 o2' /\ distinct_ops o2 o2' /\  
                     eq (merge l (do a o1) (do b o2)) (do (merge l (do a o1) b) o2))
-          (ensures eq (merge l (do a o1) (do (do b o2') o2)) (do (merge l (do a o1) (do b o2')) o2))
+          (ensures eq (merge l (do a o1) (do (do b o2') o2)) (do (merge l (do a o1) (do b o2')) o2)) = ()
 
-val rc_ind_left (l a b:concrete_st) (o1 o2 o1':op_t)
+let rc_ind_left (l a b:concrete_st) (o1 o2 o1':op_t)
   : Lemma (requires Fst_then_snd? (rc o1 o2) /\
                     distinct_ops o1 o2 /\ distinct_ops o1 o1' /\ distinct_ops o2 o1' /\
                     eq (merge l (do a o1) (do b o2)) (do (merge l (do a o1) b) o2))
-          (ensures eq (merge l (do (do a o1') o1) (do b o2)) (do (merge l (do (do a o1') o1) b) o2))
+          (ensures eq (merge l (do (do a o1') o1) (do b o2)) (do (merge l (do (do a o1') o1) b) o2)) = ()
 
 //Special case of rc_intermediate_v1
-val rc_ind_lca (l:concrete_st) (o1 o2 o:op_t)
+let rc_ind_lca (l:concrete_st) (o1 o2 o:op_t)
   : Lemma (requires Fst_then_snd? (rc o1 o2) /\ 
                     distinct_ops o1 o2 /\ distinct_ops o o1 /\ distinct_ops o o2 /\
                     eq (merge l (do l o1) (do l o2)) (do (do l o1) o2))
-          (ensures eq (merge (do l o) (do (do l o) o1) (do (do l o) o2)) (do (do (do l o) o1) o2))
+          (ensures eq (merge (do l o) (do (do l o) o1) (do (do l o) o2)) (do (do (do l o) o1) o2)) = ()
 
-val rc_base (o1 o2:op_t)
+let rc_base (o1 o2:op_t)
   : Lemma (requires Fst_then_snd? (rc o1 o2) /\ distinct_ops o1 o2)
-          (ensures eq (merge init_st (do init_st o1) (do init_st o2)) (do (do init_st o1) o2))
+          (ensures eq (merge init_st (do init_st o1) (do init_st o2)) (do (do init_st o1) o2)) = ()
 
-val rc_inter_base_right (l a b c:concrete_st) (o1 o2 ob ol:op_t) 
+let rc_inter_base_right (l a b c:concrete_st) (o1 o2 ob ol:op_t) 
   : Lemma (requires Fst_then_snd? (rc o1 o2) /\ Fst_then_snd? (rc ob ol) /\ 
                     distinct_ops o1 o2 /\ distinct_ops o1 ob /\ distinct_ops o1 ol /\ distinct_ops o2 ob /\ distinct_ops o2 ol /\ distinct_ops ob ol /\ 
                     eq (merge (do l ol) (do (do a ol) o1) (do (do b ol) o2)) (do (do (do c ol) o1) o2) /\
                     eq (merge l (do a o1) (do b o2)) (do (do c o1) o2) /\
                     eq (merge l (do a ol) (do b ob)) (do (do c ob) ol)) //***EXTRA***
-          (ensures eq (merge (do l ol) (do (do a ol) o1) (do (do (do b ob) ol) o2)) (do (do (do (do c ob) ol) o1) o2))
+          (ensures eq (merge (do l ol) (do (do a ol) o1) (do (do (do b ob) ol) o2)) (do (do (do (do c ob) ol) o1) o2)) = ()
 
-val rc_inter_base_left (l a b c:concrete_st) (o1 o2 ob ol:op_t) 
+let rc_inter_base_left (l a b c:concrete_st) (o1 o2 ob ol:op_t) 
   : Lemma (requires Fst_then_snd? (rc o1 o2) /\ Fst_then_snd? (rc ob ol) /\ 
                     distinct_ops o1 o2 /\ distinct_ops o1 ob /\ distinct_ops o1 ol /\ distinct_ops o2 ob /\ distinct_ops o2 ol /\ distinct_ops ob ol /\ 
                     eq (merge (do l ol) (do (do a ol) o1) (do (do b ol) o2)) (do (do (do c ol) o1) o2) /\
                     eq (merge l (do a o1) (do b o2)) (do (do c o1) o2) /\
                     eq (merge l (do a ob) (do b ol)) (do (do c ob) ol)) //***EXTRA***
-          (ensures eq (merge (do l ol) (do (do (do a ob) ol) o1) (do (do b ol) o2)) (do (do (do (do c ob) ol) o1) o2))
+          (ensures eq (merge (do l ol) (do (do (do a ob) ol) o1) (do (do b ol) o2)) (do (do (do (do c ob) ol) o1) o2)) = ()
           
-val rc_inter_right (l a b c:concrete_st) (o1 o2 ob ol o:op_t)
+let rc_inter_right (l a b c:concrete_st) (o1 o2 ob ol o:op_t)
   : Lemma (requires Fst_then_snd? (rc o1 o2) /\ Fst_then_snd? (rc ob ol) /\ 
                     distinct_ops o1 o2 /\ distinct_ops o1 ob /\ distinct_ops o1 ol /\ distinct_ops o1 o /\ distinct_ops o2 ob /\ 
                     distinct_ops o2 ol /\ distinct_ops o2 o /\ distinct_ops ob ol /\ distinct_ops ob o /\ distinct_ops ol o /\
                     get_rid o <> get_rid ol (*o,ol must be concurrent*) /\
                     ((~ (commutes_with o ob)) \/ Fst_then_snd? (rc o ol)) /\
                     eq (merge (do l ol) (do (do a ol) o1) (do (do (do b ob) ol) o2)) (do (do (do (do c ob) ol) o1) o2))
-      (ensures eq (merge (do l ol) (do (do a ol) o1) (do (do (do (do b o) ob) ol) o2)) (do (do (do (do (do c o) ob) ol) o1) o2))
+      (ensures eq (merge (do l ol) (do (do a ol) o1) (do (do (do (do b o) ob) ol) o2)) (do (do (do (do (do c o) ob) ol) o1) o2)) = ()
 
-val rc_inter_left (l a b c:concrete_st) (o1 o2 ob ol o:op_t)
+let rc_inter_left (l a b c:concrete_st) (o1 o2 ob ol o:op_t)
   : Lemma (requires Fst_then_snd? (rc o1 o2) /\ Fst_then_snd? (rc ob ol) /\ 
                     distinct_ops o1 o2 /\ distinct_ops o1 ob /\ distinct_ops o1 ol /\ distinct_ops o1 o /\ distinct_ops o2 ob /\ 
                     distinct_ops o2 ol /\ distinct_ops o2 o /\ distinct_ops ob ol /\ distinct_ops ob o /\ distinct_ops ol o /\
                     get_rid o <> get_rid ol (*o,ol must be concurrent*) /\
                     ((~ (commutes_with o ob)) \/ Fst_then_snd? (rc o ol)) /\
                     eq (merge (do l ol) (do (do (do a ob) ol) o1) (do (do b ol) o2)) (do (do (do (do c ob) ol) o1) o2))
-      (ensures eq (merge (do l ol) (do (do (do (do a o) ob) ol) o1) (do (do b ol) o2)) (do (do (do (do (do c o) ob) ol) o1) o2))
+      (ensures eq (merge (do l ol) (do (do (do (do a o) ob) ol) o1) (do (do b ol) o2)) (do (do (do (do (do c o) ob) ol) o1) o2)) = ()
 
 // In general, the events ol,oi, below should be such that these exists o, (rc o ol), (rc o oi)
-val rc_inter_lca (l a b c:concrete_st) (o1 o2 ol oi:op_t)
+let rc_inter_lca (l a b c:concrete_st) (o1 o2 ol oi:op_t)
   : Lemma (requires distinct_ops o1 o2 /\ Fst_then_snd? (rc o1 o2) /\ 
                     (exists o. Fst_then_snd? (rc o ol)) /\ 
                     (exists o. Fst_then_snd? (rc o oi)) /\ 
                     eq (merge (do l oi) (do (do a oi) o1) (do (do b oi) o2)) (do (do (do c oi) o1) o2) /\
                     eq (merge (do l ol) (do (do a ol) o1) (do (do b ol) o2)) (do (do (do c ol) o1) o2))
-    (ensures eq (merge (do (do l oi) ol) (do (do (do a oi) ol) o1) (do (do (do b oi) ol) o2)) (do (do (do (do c oi) ol) o1) o2))
+    (ensures eq (merge (do (do l oi) ol) (do (do (do a oi) ol) o1) (do (do (do b oi) ol) o2)) (do (do (do (do c oi) ol) o1) o2)) = ()
 
 (*One op*)
 ///////////////
-val one_op_ind_right (l a b c:concrete_st) (o2 o2':op_t)
+let one_op_ind_right (l a b c:concrete_st) (o2 o2':op_t)
    : Lemma (requires eq (merge l a (do b o2)) (do (merge l a b) o2))
-           (ensures eq (merge l a (do (do b o2') o2)) (do (merge l a (do b o2')) o2))
+           (ensures eq (merge l a (do (do b o2') o2)) (do (merge l a (do b o2')) o2)) = ()
 
-val one_op_ind_left (l a b c:concrete_st) (o1 o1':op_t)
+let one_op_ind_left (l a b c:concrete_st) (o1 o1':op_t)
    : Lemma (requires eq (merge l (do a o1) b) (do (merge l a b) o1))
-           (ensures eq (merge l (do (do a o1') o1) b) (do (merge l (do a o1') b) o1))
+           (ensures eq (merge l (do (do a o1') o1) b) (do (merge l (do a o1') b) o1)) = ()
            
-val one_op_ind_lca (l:concrete_st) (o2 o:op_t)
+let one_op_ind_lca (l:concrete_st) (o2 o:op_t)
   : Lemma (requires eq (merge l l (do l o2)) (do l o2))
-          (ensures eq (merge (do l o) (do l o) (do (do l o) o2)) (do (do l o) o2)) 
+          (ensures eq (merge (do l o) (do l o) (do (do l o) o2)) (do (do l o) o2)) = () 
 
-val one_op_base (o2:op_t)
-  : Lemma (ensures eq (merge init_st init_st (do init_st o2)) (do init_st o2))
+let one_op_base (o2:op_t)
+  : Lemma (ensures eq (merge init_st init_st (do init_st o2)) (do init_st o2)) = ()
 
-val one_op_inter_base_right (l a b c:concrete_st) (o2 ob ol:op_t) 
+let one_op_inter_base_right (l a b c:concrete_st) (o2 ob ol:op_t) 
   : Lemma (requires Fst_then_snd? (rc ob ol) /\
                     distinct_ops o2 ob /\ distinct_ops o2 ol /\ distinct_ops ob ol /\
                     eq (merge (do l ol) (do a ol) (do (do b ol) o2)) (do (do c ol) o2) /\
                     eq (merge l a (do b o2)) (do c o2) /\
                     eq (merge l (do a ol) (do b ob)) (do (do c ob) ol)) //***EXTRA***
-          (ensures eq (merge (do l ol) (do a ol) (do (do (do b ob) ol) o2)) (do (do (do c ob) ol) o2))
+          (ensures eq (merge (do l ol) (do a ol) (do (do (do b ob) ol) o2)) (do (do (do c ob) ol) o2)) = ()
 
-val one_op_inter_base_left (l a b c:concrete_st) (o2 ob ol:op_t) 
+let one_op_inter_base_left (l a b c:concrete_st) (o2 ob ol:op_t) 
   : Lemma (requires Fst_then_snd? (rc ob ol) /\
                     distinct_ops o2 ob /\ distinct_ops o2 ol /\ distinct_ops ob ol /\
                     eq (merge (do l ol) (do a ol) (do (do b ol) o2)) (do (do c ol) o2) /\
@@ -185,82 +199,82 @@ val one_op_inter_base_left (l a b c:concrete_st) (o2 ob ol:op_t)
                     eq (merge l a (do b o2)) (do c o2) /\
                     eq (merge l (do a ol) (do b ob)) (do (do c ob) ol) /\ //***EXTRA***
                     eq (merge l (do (do a ob) ol) (do b ol)) (do (do c ob) ol)) //***EXTRA***
-          (ensures eq (merge (do l ol) (do (do a ob) ol) (do (do b ol) o2)) (do (do (do c ob) ol) o2))
+          (ensures eq (merge (do l ol) (do (do a ob) ol) (do (do b ol) o2)) (do (do (do c ob) ol) o2)) = ()
 
-val one_op_inter_right (l a b c:concrete_st) (o2 ob ol o:op_t) 
+let one_op_inter_right (l a b c:concrete_st) (o2 ob ol o:op_t) 
   : Lemma (requires Fst_then_snd? (rc ob ol) /\
                     distinct_ops o ob /\ distinct_ops o ol /\ distinct_ops o ol /\ distinct_ops ob ol /\ distinct_ops ob o2 /\ distinct_ops o2 ol /\
                     get_rid o <> get_rid ol (*o,ol must be concurrent*) /\
                     ((~ (commutes_with o ob)) \/ Fst_then_snd? (rc o ol)) /\
                     eq (merge (do l ol) (do a ol) (do (do (do b ob) ol) o2)) (do (do (do c ob) ol) o2))
-          (ensures eq (merge (do l ol) (do a ol) (do (do (do (do b o) ob) ol) o2)) (do (do (do (do c o) ob) ol) o2))
+          (ensures eq (merge (do l ol) (do a ol) (do (do (do (do b o) ob) ol) o2)) (do (do (do (do c o) ob) ol) o2)) = ()
           
-val one_op_inter_left (l a b c:concrete_st) (o2 ob ol o:op_t) 
+let one_op_inter_left (l a b c:concrete_st) (o2 ob ol o:op_t) 
   : Lemma (requires Fst_then_snd? (rc ob ol) /\
                     distinct_ops o ob /\ distinct_ops o ol /\ distinct_ops o ol /\ distinct_ops ob ol /\ distinct_ops ob o2 /\ distinct_ops o2 ol /\
                     get_rid o <> get_rid ol (*o,ol must be concurrent*) /\
                     ((~ (commutes_with o ob)) \/ Fst_then_snd? (rc o ol)) /\
                     eq (merge (do l ol) (do (do a ob) ol) (do (do b ol) o2)) (do (do (do c ob) ol) o2))
-          (ensures eq (merge (do l ol) (do (do (do a o) ob) ol) (do (do b ol) o2)) (do (do (do (do c o) ob) ol) o2))
+          (ensures eq (merge (do l ol) (do (do (do a o) ob) ol) (do (do b ol) o2)) (do (do (do (do c o) ob) ol) o2)) = ()
 
 // In general, the events o',o_n, below should be such that these exists o, (rc o o')
-val one_op_inter_lca (l a b c:concrete_st) (o2 ol oi:op_t)
+let one_op_inter_lca (l a b c:concrete_st) (o2 ol oi:op_t)
   : Lemma (requires (exists o. Fst_then_snd? (rc o ol)) /\ 
                     (exists o. Fst_then_snd? (rc o oi)) /\ 
                     eq (merge (do l oi) (do a oi) (do (do b oi) o2)) (do (do c oi) o2) /\
                     eq (merge (do l ol) (do a ol) (do (do b ol) o2)) (do (do c ol) o2))
-          (ensures eq (merge (do (do l oi) ol) (do (do a oi) ol) (do (do (do b oi) ol) o2)) (do (do (do c oi) ol) o2))
+          (ensures eq (merge (do (do l oi) ol) (do (do a oi) ol) (do (do (do b oi) ol) o2)) (do (do (do c oi) ol) o2)) = ()
 
 (*Zero op *)
 ///////////////
 // because we proved that e_i^l rcp eb is not possible.
 //e_i^l vis eb is not possible
 // so either eb rcp e_i^l or eb rct e_i^l is possible
-val zero_op_inter_base_right (l a b c:concrete_st) (ob ol:op_t) 
+let zero_op_inter_base_right (l a b c:concrete_st) (ob ol:op_t) 
   : Lemma (requires Fst_then_snd? (rc ob ol) /\ distinct_ops ob ol /\ 
                     eq (merge (do l ol) (do a ol) (do b ol)) (do c ol) /\
                     eq (merge l a b) c /\
                     eq (merge l (do a ol) (do b ob)) (do (do c ob) ol)) //***EXTRA***
-          (ensures eq (merge (do l ol) (do a ol) (do (do b ob) ol)) (do (do c ob) ol)) 
+          (ensures eq (merge (do l ol) (do a ol) (do (do b ob) ol)) (do (do c ob) ol)) = () 
 
-val zero_op_inter_base_left (l a b c:concrete_st) (ob ol:op_t) 
+let zero_op_inter_base_left (l a b c:concrete_st) (ob ol:op_t) 
   : Lemma (requires Fst_then_snd? (rc ob ol) /\ distinct_ops ob ol /\ 
                     eq (merge (do l ol) (do a ol) (do b ol)) (do c ol) /\
                     eq (merge l a b) c /\
                     eq (merge l (do a ob) (do b ol)) (do (do c ob) ol)) //***EXTRA***
-          (ensures eq (merge (do l ol) (do (do a ob) ol) (do b ol) ) (do (do c ob) ol)) 
+          (ensures eq (merge (do l ol) (do (do a ob) ol) (do b ol) ) (do (do c ob) ol)) = () 
 
-val zero_op_inter_right (l a b c:concrete_st) (ob ol o:op_t)
+let zero_op_inter_right (l a b c:concrete_st) (ob ol o:op_t)
   : Lemma (requires Fst_then_snd? (rc ob ol) /\ distinct_ops ob ol /\ 
                     get_rid o <> get_rid ol (*o,ol must be concurrent*) /\
                     ((~ (commutes_with o ob)) \/ Fst_then_snd? (rc o ol)) /\
                     eq (merge (do l ol) (do a ol) (do (do b ob) ol)) (do (do c ob) ol))
-          (ensures eq (merge (do l ol) (do a ol) (do (do (do b o) ob) ol)) (do (do (do c o) ob) ol)) 
+          (ensures eq (merge (do l ol) (do a ol) (do (do (do b o) ob) ol)) (do (do (do c o) ob) ol)) = ()
 
-val zero_op_inter_left (l a b c:concrete_st) (ob ol o:op_t)
+let zero_op_inter_left (l a b c:concrete_st) (ob ol o:op_t)
   : Lemma (requires Fst_then_snd? (rc ob ol) /\ distinct_ops ob ol /\ 
                     get_rid o <> get_rid ol (*o,ol must be concurrent*) /\
                     ((~ (commutes_with o ob)) \/ Fst_then_snd? (rc o ol)) /\
                     eq (merge (do l ol) (do (do a ob) ol) (do b ol)) (do (do c ob) ol))
-          (ensures eq (merge (do l ol) (do (do (do a o) ob) ol) (do b ol)) (do (do (do c o) ob) ol)) 
+          (ensures eq (merge (do l ol) (do (do (do a o) ob) ol) (do b ol)) (do (do (do c o) ob) ol)) = ()
 
 // In general, the event "o" below should be such that these exists o', (rc o' o)
-val zero_op_inter_lca_v1 (l a b c:concrete_st) (ol:op_t)
+let zero_op_inter_lca_v1 (l a b c:concrete_st) (ol:op_t)
   : Lemma (requires (exists o'. Fst_then_snd? (rc o' ol)) /\ eq (merge l a b) c)
-          (ensures eq (merge (do l ol) (do a ol) (do b ol)) (do c ol))
+          (ensures eq (merge (do l ol) (do a ol) (do b ol)) (do c ol)) = ()
 
 // In general, the events o',o_n, below should be such that these exists o, (rc o o')
-val zero_op_inter_lca_v2 (l a b c:concrete_st) (ol oi:op_t)
+let zero_op_inter_lca_v2 (l a b c:concrete_st) (ol oi:op_t)
   : Lemma (requires (exists o. Fst_then_snd? (rc o ol)) /\ 
                     (exists o. Fst_then_snd? (rc o oi)) /\
                     eq (merge (do l oi) (do a oi) (do b oi)) (do c oi)  /\
                     eq (merge (do l ol) (do a ol) (do b ol)) (do c ol))
-          (ensures eq (merge (do (do l oi) ol) (do (do a oi) ol) (do (do b oi) ol)) (do (do c oi) ol))
+          (ensures eq (merge (do (do l oi) ol) (do (do a oi) ol) (do (do b oi) ol)) (do (do c oi) ol)) = ()
 
 (* 2 op Comm  *)
 ///////////////////
 
-val comm_ind_right (l a b c:concrete_st) (o1 o2 o2':op_t)
+let comm_ind_right (l a b c:concrete_st) (o1 o2 o2':op_t)
   : Lemma (requires Either? (rc o1 o2) /\ 
                     distinct_ops o1 o2 /\ distinct_ops o1 o2' /\ distinct_ops o2 o2' /\
                     eq (merge l (do a o1) (do b o2)) (do (do (merge l a b) o2) o1) /\
@@ -269,9 +283,9 @@ val comm_ind_right (l a b c:concrete_st) (o1 o2 o2':op_t)
                     ~ (Fst_then_snd? (rc o1 o2')) /\
                     ~ (exists o3 b'. eq (do (do b o2') o2) (do b' o3) /\ distinct_ops o1 o3 /\ Fst_then_snd? (rc o1 o3)) /\
                     ~ (exists o3 b'. eq (do b o2) (do b' o3) /\ distinct_ops o1 o3 /\ Fst_then_snd? (rc o1 o3)))                    
-          (ensures eq (merge l (do a o1) (do (do b o2') o2)) (do (do (merge l a (do b o2')) o2) o1))
+          (ensures eq (merge l (do a o1) (do (do b o2') o2)) (do (do (merge l a (do b o2')) o2) o1)) = ()
 
-val comm_ind_left (l a b c:concrete_st) (o1 o2 o1':op_t)
+let comm_ind_left (l a b c:concrete_st) (o1 o2 o1':op_t)
   : Lemma (requires Either? (rc o1 o2) /\ 
                     distinct_ops o1 o2 /\ distinct_ops o1 o1' /\ distinct_ops o2 o1' /\
                     eq (merge l (do a o1) (do b o2)) (do (do (merge l a b) o2) o1) /\
@@ -280,37 +294,37 @@ val comm_ind_left (l a b c:concrete_st) (o1 o2 o1':op_t)
                     ~ (Fst_then_snd? (rc o2 o1')) /\
                     ~ (exists o3 b'. eq (do (do b o1') o2) (do b' o3) /\ distinct_ops o1 o3 /\ Fst_then_snd? (rc o1 o3)) /\
                     ~ (exists o3 b'. eq (do b o2) (do b' o3) /\ distinct_ops o1 o3 /\ Fst_then_snd? (rc o1 o3)))                    
-          (ensures eq (merge l (do (do a o1') o1) (do b o2)) (do (do (merge l (do a o1') b) o2) o1))
+          (ensures eq (merge l (do (do a o1') o1) (do b o2)) (do (do (merge l (do a o1') b) o2) o1)) = ()
 
-val comm_ind_lca (l:concrete_st) (o1 o2 ol:op_t)
+let comm_ind_lca (l:concrete_st) (o1 o2 ol:op_t)
   : Lemma (requires Either? (rc o1 o2) /\ 
                     distinct_ops o1 o2 /\ distinct_ops o1 ol /\ distinct_ops o2 ol /\
                     eq (merge l (do l o1) (do l o2)) (do (do l o2) o1))
-          (ensures eq (merge (do l ol) (do (do l ol) o1) (do (do l ol) o2)) (do (do (do l ol) o2) o1))
+          (ensures eq (merge (do l ol) (do (do l ol) o1) (do (do l ol) o2)) (do (do (do l ol) o2) o1)) = ()
 
-val comm_base (o1 o2:op_t)
+let comm_base (o1 o2:op_t)
   : Lemma (requires Either? (rc o1 o2) /\ distinct_ops o1 o2)
-          (ensures eq (merge init_st (do init_st o1) (do init_st o2)) (do (do init_st o1) o2))
+          (ensures eq (merge init_st (do init_st o1) (do init_st o2)) (do (do init_st o1) o2)) = ()
 
-val comm_inter_base_right (l a b c:concrete_st) (o1 o2 ob ol:op_t) 
+let comm_inter_base_right (l a b c:concrete_st) (o1 o2 ob ol:op_t) 
   : Lemma (requires Either? (rc o1 o2) /\ Fst_then_snd? (rc ob ol) /\ 
                     distinct_ops o1 o2 /\ distinct_ops o1 ob /\ distinct_ops o1 ol /\ distinct_ops o2 ob /\ distinct_ops o2 ol /\ distinct_ops ob ol /\
                     eq (merge (do l ol) (do (do a ol) o1) (do (do b ol) o2)) (do (do (do c ol) o1) o2) /\ 
                     eq (merge l (do a o1) (do b o2)) (do (do c o1) o2) /\
                     eq (merge l (do a o1) (do (do b ob) o2)) (do (do (merge l a (do b ob)) o1) o2) /\ //comes from comm_ind_right
                     eq (merge (do l ol) (do a ol) (do (do b ob) ol)) (do (do c ob) ol)) //comes from intermediate_base_zero_op
-          (ensures eq (merge (do l ol) (do (do a ol) o1) (do (do (do b ob) ol) o2)) (do (do (do (do c ob) ol) o1) o2))
+          (ensures eq (merge (do l ol) (do (do a ol) o1) (do (do (do b ob) ol) o2)) (do (do (do (do c ob) ol) o1) o2)) = ()
 
-val comm_inter_base_left (l a b c:concrete_st) (o1 o2 ob ol:op_t) 
+let comm_inter_base_left (l a b c:concrete_st) (o1 o2 ob ol:op_t) 
   : Lemma (requires Either? (rc o1 o2) /\ Fst_then_snd? (rc ob ol) /\ 
                     distinct_ops o1 o2 /\ distinct_ops o1 ob /\ distinct_ops o1 ol /\ distinct_ops o2 ob /\ distinct_ops o2 ol /\ distinct_ops ob ol /\
                     eq (merge (do l ol) (do (do a ol) o1) (do (do b ol) o2)) (do (do (do c ol) o1) o2) /\ 
                     eq (merge l (do a o1) (do b o2)) (do (do c o1) o2) /\
                     eq (merge l (do (do a ob) o1) (do b o2)) (do (do (merge l (do a ob) b) o1) o2) /\ //comes from comm_ind_left
                     eq (merge (do l ol) (do (do a ob) ol) (do b ol)) (do (do c ob) ol)) //comes from intermediate_base_zero_op
-          (ensures eq (merge (do l ol) (do (do (do a ob) ol) o1) (do (do b ol) o2)) (do (do (do (do c ob) ol) o1) o2))
+          (ensures eq (merge (do l ol) (do (do (do a ob) ol) o1) (do (do b ol) o2)) (do (do (do (do c ob) ol) o1) o2)) = ()
 
-val comm_inter_right (l a b c:concrete_st) (o1 o2 ob ol o:op_t)
+let comm_inter_right (l a b c:concrete_st) (o1 o2 ob ol o:op_t)
   : Lemma (requires Either? (rc o1 o2) /\ Fst_then_snd? (rc ob ol) /\ 
                     distinct_ops o1 o2 /\ distinct_ops o1 ob /\ distinct_ops o1 ol /\ distinct_ops o1 o /\ distinct_ops o2 ob /\ 
                     distinct_ops o2 ol /\ distinct_ops o2 o /\ distinct_ops ob ol /\ distinct_ops ob o /\ distinct_ops ol o /\
@@ -318,9 +332,9 @@ val comm_inter_right (l a b c:concrete_st) (o1 o2 ob ol o:op_t)
                     //Either? (rc o ol) /\ 
                     ((~ (commutes_with o ob)) \/ Fst_then_snd? (rc o ol)) /\
                     eq (merge (do l ol) (do (do a ol) o1) (do (do (do b ob) ol) o2)) (do (do (do (do c ob) ol) o1) o2))
-          (ensures eq (merge (do l ol) (do (do a ol) o1) (do (do (do (do b o) ob) ol) o2)) (do (do (do (do (do c o) ob) ol) o1) o2))
+          (ensures eq (merge (do l ol) (do (do a ol) o1) (do (do (do (do b o) ob) ol) o2)) (do (do (do (do (do c o) ob) ol) o1) o2)) = ()
 
-val comm_inter_left (l a b c:concrete_st) (o1 o2 ob ol o:op_t)
+let comm_inter_left (l a b c:concrete_st) (o1 o2 ob ol o:op_t)
   : Lemma (requires Either? (rc o1 o2) /\ Fst_then_snd? (rc ob ol) /\ 
                     distinct_ops o1 o2 /\ distinct_ops o1 ob /\ distinct_ops o1 ol /\ distinct_ops o1 o /\ distinct_ops o2 ob /\ 
                     distinct_ops o2 ol /\ distinct_ops o2 o /\ distinct_ops ob ol /\ distinct_ops ob o /\ distinct_ops ol o /\
@@ -328,72 +342,47 @@ val comm_inter_left (l a b c:concrete_st) (o1 o2 ob ol o:op_t)
                     //Either? (rc o ol) /\ 
                     ((~ (commutes_with o ob)) \/ Fst_then_snd? (rc o ol)) /\
                     eq (merge (do l ol) (do (do (do a ob) ol) o1) (do (do b ol) o2)) (do (do (do (do c ob) ol) o1) o2))
-          (ensures eq (merge (do l ol) (do (do (do (do a o) ob) ol) o1) (do (do b ol) o2)) (do (do (do (do (do c o) ob) ol) o1) o2))
+          (ensures eq (merge (do l ol) (do (do (do (do a o) ob) ol) o1) (do (do b ol) o2)) (do (do (do (do (do c o) ob) ol) o1) o2)) = ()
 
-val comm_inter_lca (l a b c:concrete_st) (o1 o2 ol:op_t)
+let comm_inter_lca (l a b c:concrete_st) (o1 o2 ol:op_t)
   : Lemma (requires Either? (rc o1 o2) /\ 
                     distinct_ops o1 o2 /\ distinct_ops o1 ol /\ distinct_ops ol o2 /\
                     (exists o'. Fst_then_snd? (rc o' ol)) /\
                     eq (merge l (do a o1) (do b o2)) (do (do c o1) o2))
-          (ensures eq (merge (do l ol) (do (do a ol) o1) (do (do b ol) o2)) (do (do (do c ol) o1) o2))
+          (ensures eq (merge (do l ol) (do (do a ol) o1) (do (do b ol) o2)) (do (do (do c ol) o1) o2)) = ()
 
 ////////////////////////////////////////////////////////////////
 //// Sequential implementation //////
 
 // the concrete state 
-val concrete_st_s : Type0
+let concrete_st_s = bool & bool
 
 // init state 
-val init_st_s : concrete_st_s
+let init_st_s = (false, false)
 
 // apply an operation to a state 
-val do_s (st_s:concrete_st_s) (_:op_t) : concrete_st_s
+let do_s (st_s:concrete_st_s) (o:op_t) =
+  match snd (snd o) with
+  |Add1 -> (true, snd st_s)
+  |Add2 -> (fst st_s, true)
+  |Rem1 -> (false, snd st_s)
+  |Rem2 -> (fst st_s, false)
 
 // equivalence relation between the concrete states of sequential type and MRDT
-val eq_sm (st_s:concrete_st_s) (st:concrete_st) : Type0
+let eq_sm (st_s:concrete_st_s) (st:concrete_st) =
+  (fst (st_s) = false <==> (exists e. S.mem e st /\ snd e = 1)) /\
+  (snd (st_s) = false <==> (exists e. S.mem e st /\ snd e = 2))
 
 // initial states are equivalent
-val initial_eq (_:unit)
-  : Lemma (ensures eq_sm init_st_s init_st)
+let initial_eq (_:unit)
+  : Lemma (ensures eq_sm init_st_s init_st) = ()
 
 // equivalence between states of sequential type and MRDT at every operation
-val do_eq (st_s:concrete_st_s) (st:concrete_st) (op:op_t)
+let do_eq (st_s:concrete_st_s) (st:concrete_st) (op:op_t)
   : Lemma (requires eq_sm st_s st)
-          (ensures eq_sm (do_s st_s op) (do st op))
+          (ensures eq_sm (do_s st_s op) (do st op)) = 
+  assert (Rem1? (snd (snd op)) ==> S.mem (fst op, 1) (do st op)); 
+  assert (Rem2? (snd (snd op)) ==> S.mem (fst op, 2) (do st op)); 
+  ()
 
-////////////////////////////////////////////////////////////////
-
-////////////////////////////////////////////////////////////////
-////Equivalence of  MRDT & Sequential implementation  //////
-
-// the concrete state 
-(*val concrete_st_s : Type0
-
-// init state 
-val init_st_s : concrete_st_s
-
-// apply an operation to a state 
-val do_s (st_s:concrete_st_s) (_:op_t) : concrete_st_s
-
-//query type
-val query_t : eqtype
-
-//ret type
-val ret_t : Type0
-
-//query return value - MRDT
-val query_m (s:concrete_st) (q:query_t) : ret_t
-
-//query return value - Seq impl
-val query_s (s:concrete_st_s) (q:query_t) : ret_t
-
-// initial states are equivalent
-val initial_eq (q:query_t)
-  : Lemma (ensures query_s init_st_s q == query_m init_st q)
-
-//equivalence between states of sequential type and MRDT at every operation
-val do_eq (st_s:concrete_st_s) (st:concrete_st) (op:op_t) (q:query_t)
-  : Lemma (requires query_s st_s q == query_m st q)
-          (ensures query_s (do_s st_s op) q == query_m (do st op) q)*)
-         
 ////////////////////////////////////////////////////////////////
